SeqPL/Formula/Countable.lean
@@ -1,0 +1,45 @@
+module
+
+public import SeqPL.Formula.Basic
+public import Mathlib.Logic.Encodable.Basic
+public import Mathlib.Data.Nat.Pairing
+
+@[expose]
+public section
+
+namespace Formula
+
+variable {α : Type*} [Encodable α]
+
+/-- `Formula α` を `ℕ` へ単射符号化する． -/
+def toNat : Formula α → ℕ
+  | atom a => Nat.pair 0 (Encodable.encode a)
+  | ⊥      => Nat.pair 1 0
+  | A 🡒 B  => Nat.pair 2 (Nat.pair A.toNat B.toNat)
+  | □A     => Nat.pair 3 A.toNat
+
+lemma toNat_injective : Function.Injective (toNat : Formula α → ℕ) := by
+  suffices H : ∀ A B : Formula α, toNat A = toNat B → A = B by intro a b; exact H a b;
+  intro A;
+  induction A with
+  | atom a => intro B h; cases B <;> simp_all [toNat, Nat.pair_eq_pair, Encodable.encode_inj];
+  | bot => intro B h; cases B <;> simp_all [toNat, Nat.pair_eq_pair];
+  | imp A₁ A₂ ih1 ih2 =>
+    intro B h; cases B;
+    case imp B₁ B₂ =>
+      simp only [toNat, Nat.pair_eq_pair] at h;
+      obtain ⟨-, h1, h2⟩ := h;
+      rw [ih1 _ h1, ih2 _ h2];
+    all_goals simp [toNat, Nat.pair_eq_pair] at h;
+  | box A₁ ih =>
+    intro B h; cases B;
+    case box B₁ =>
+      simp only [toNat, Nat.pair_eq_pair] at h;
+      rw [ih _ h.2];
+    all_goals simp [toNat, Nat.pair_eq_pair] at h;
+
+instance : Countable (Formula α) := toNat_injective.countable
+
+end Formula
+
+end
