SeqPL/ProvabilityLogic/GL/Uniform.lean
@@ -1,0 +1,31 @@
+module
+
+public import SeqPL.ProvabilityLogic.GL.Basic
+
+@[expose] public section
+
+open Classical
+open LO
+open LO.FirstOrder.ProvabilityAbstraction
+
+variable {κ : Type*} [Nonempty κ]
+         {α : Type*}
+         {A B : _root_.Formula α}
+
+namespace LogicGL
+
+section
+
+variable {T : FirstOrder.ArithmeticTheory} [T.Δ₁] [𝗜𝚺₁ ⪯ T]
+
+theorem uniform_arithmetical_completeness : ∃ f : StandardRealization α T, ∀ A, T ⊢ f A ↔ A ∈ LogicGL := by sorry;
+
+protected noncomputable def uniformRealization (T : FirstOrder.ArithmeticTheory) [T.Δ₁] [𝗜𝚺₁ ⪯ T] : StandardRealization α T := uniform_arithmetical_completeness.choose
+
+lemma uniformRealization_spec : ∀ A : Formula α, T ⊢ LogicGL.uniformRealization T A ↔ A ∈ LogicGL := uniform_arithmetical_completeness.choose_spec
+
+end
+
+end LogicGL
+
+end
