SeqPL/Vorspiel/Set/Approximate.lean
@@ -1,0 +1,79 @@
+module
+
+public import Mathlib.Data.Set.Countable
+public import Mathlib.Data.Set.Finite.Range
+public import Mathlib.Data.Finset.Preimage
+public import Mathlib.Data.Fintype.Sigma
+
+@[expose]
+public section
+
+/-!
+  `Foundation.Vorspiel.Set.Basic` / `Foundation.Vorspiel.Finset.Basic` から必要な補題を移植．
+-/
+
+namespace Set
+
+variable {α : Type*} {s t : Set α} {a : α}
+
+lemma ssubset_of_subset_ne (h : s ⊆ t) (hne : s ≠ t) : s ⊂ t := by
+  constructor;
+  . assumption;
+  . revert hne;
+    contrapose!;
+    intro _;
+    apply Set.eq_of_subset_of_subset <;> assumption;
+
+/--
+  Thanks to @plp127
+
+  https://leanprover.zulipchat.com/#narrow/channel/217875-Is-there-code-for-X.3F/topic/ascending.2Fdecending.20lemmata.20related.20.60Set.60.20and.20.60Finset.60/near/539292838
+-/
+lemma infinitely_finset_approximate (count : s.Countable) (inf : s.Infinite) (ha : a ∈ s) :
+  ∃ f : ℕ → Finset α, ((f 0) = {a}) ∧ (∀ i, f i ⊂ f (i + 1)) ∧ (∀ i, ↑(f i) ⊆ s) ∧ (∀ b ∈ s, ∃ i, b ∈ f i) := by
+  let X' := s \ {a}
+  have count' : Countable X' := (count.mono Set.diff_subset).to_subtype
+  have inf' : Infinite X' := (inf.diff (Set.finite_singleton a)).to_subtype
+  obtain ⟨eq⟩ : Nonempty (Nat ≃ X') := nonempty_equiv_of_countable
+  refine ⟨
+    fun n => Finset.cons a ((Finset.range n).map
+    (eq.toEmbedding.trans (Function.Embedding.subtype _))) ?_, ?_, ?_, ?_, ?_
+  ⟩
+  · suffices ∀ x < n, ¬↑(eq x) = a by simpa;
+    intro x _
+    exact (eq x).prop.right
+  · rfl
+  · simp [Finset.ssubset_def]
+  · suffices ∀ (i : ℕ), Set.Iio i ⊆ (fun a ↦ ↑(eq a)) ⁻¹' s by simpa [Set.insert_subset_iff, ha]
+    intro i x _;
+    exact (eq x).prop.left
+  · intro b hb
+    by_cases hba : b = a
+    · exact ⟨0, by simp [hba]⟩
+    · refine ⟨eq.symm ⟨b, hb, hba⟩ + 1, ?_⟩
+      apply Finset.mem_cons_of_mem;
+      suffices ∃ a_1 < eq.symm ⟨b, _⟩ + 1, ↑(eq _) = b by simpa;
+      exact ⟨eq.symm ⟨b, hb, hba⟩, by simp⟩
+
+end Set
+
+
+namespace Finset
+
+variable {α : Type*}
+
+/--
+  Thanks to @plp127
+
+  https://leanprover.zulipchat.com/#narrow/channel/217875-Is-there-code-for-X.3F/topic/ascending.2Fdecending.20lemmata.20related.20.60Set.60.20and.20.60Finset.60/near/539367015
+-/
+lemma no_ssubset_descending_chain {f : ℕ → Finset α} : ¬(∀ i, ∃ j > i, f j ⊂ f i) := by
+  intro h
+  have n := 0
+  induction hf : f n using WellFoundedLT.fix generalizing n with subst hf | _ _ ih
+  obtain ⟨m, -, hy⟩ := h n
+  exact ih (f m) hy m rfl
+
+end Finset
+
+end
